Improve the parser combinators library, parse handle resource uri

theories/Parser.v
@@ -1,12 +1,126 @@
-From Coq Require Export String Ascii.
+From Coq Require Export String Ascii Lia Program.Wf.
+From Coq Require List.
 From Prelude Require Export Control.
-From Prelude Require Import State Classes Either Equality.
+From Prelude Require Import State Classes Sum Equality Option.
+
+Generalizable All Variables.
 
 #[global] Open Scope monad_scope.
+
+Notation "x '>>' y" := (x >>= fun _ => y) (at level 74, right associativity).
+Notation "x '<*' y" := (x >>= fun r => (y >> pure r)) (at level 74, right associativity).
+Notation "x '*>' y" := (x >> y) (at level 74, right associativity).
 
 Definition error_stack := list string.
 
 Definition parser (a : Type) := state_t string (sum error_stack) a.
+
+Definition parse {a} (parser : parser a) (input : string) : error_stack + a :=
+  fst <$> (parser input).
+
+Class Parser {a} (p : parser a) : Prop :=
+  { is_parser (input : string) :
+      match p input with
+      | inl _ => True
+      | inr (_, output) => length output <= length input
+      end
+  }.
+
+Class StrictParser {a} (p : parser a) : Prop :=
+  { is_strict (input : string) :
+      match p input with
+      | inl _ => True
+      | inr (_, output) => length output < length input
+      end
+  }.
+
+#[program]
+Instance strict_parser {a} (p : parser a) `{StrictParser a p}
+  : Parser p.
+
+Next Obligation.
+  destruct H as [is_strict].
+  specialize is_strict with input.
+  destruct (p input) as [_|[x res]]; lia.
+Qed.
+
+#[program]
+Instance bind_parser {a b} (p : parser a) (f : a -> parser b) `{Parser a p} `{forall x, Parser (f x)}
+  : Parser (p >>= f).
+
+Next Obligation.
+  case_eq (p input).
+  + now cbn.
+  + intros [y input'] equ.
+    assert (length input' <= length input). {
+      destruct H as [is_parse].
+      specialize is_parse with input.
+      now rewrite equ in is_parse.
+    }
+    cbn.
+    case_eq (f y input').
+    ++ auto.
+    ++ intros [z output] equ'.
+       assert (length output <= length input'). {
+         specialize H0 with y.
+         destruct H0 as [is_parser].
+         specialize is_parser with input'.
+         now rewrite equ' in is_parser.
+       }
+       lia.
+Qed.
+
+#[program]
+Instance bind_strict_1 {a b} (p : parser a) (f : a -> parser b) `{StrictParser a p} `{forall x, Parser (f x)}
+  : StrictParser (p >>= f).
+
+Next Obligation.
+  case_eq (p input).
+  + now cbn.
+  + intros [y input'] equ.
+    assert (length input' < length input). {
+      destruct H as [is_strict].
+      specialize is_strict with input.
+      now rewrite equ in is_strict.
+    }
+    cbn.
+    case_eq (f y input').
+    ++ auto.
+    ++ intros [z output] equ'.
+       assert (length output <= length input'). {
+         specialize H0 with y.
+         destruct H0 as [is_parser].
+         specialize is_parser with input'.
+         now rewrite equ' in is_parser.
+       }
+       lia.
+Qed.
+
+#[program]
+Instance bind_strict_2 {a b} (p : parser a) (f : a -> parser b) `{Parser a p} `{forall x, StrictParser (f x)}
+  : StrictParser (p >>= f).
+
+Next Obligation.
+  case_eq (p input).
+  + now cbn.
+  + intros [y input'] equ.
+    assert (length input' <= length input). {
+      destruct H as [is_parser].
+      specialize is_parser with input.
+      now rewrite equ in is_parser.
+    }
+    cbn.
+    case_eq (f y input').
+    ++ auto.
+    ++ intros [z output] equ'.
+       assert (length output < length input'). {
+         specialize H0 with y.
+         destruct H0 as [is_strict].
+         specialize is_strict with input'.
+         now rewrite equ' in is_strict.
+       }
+       lia.
+Qed.
 
 Definition with_context {a} (msg : string) (p : parser a) : parser a :=
   fun input =>
@@ -15,90 +129,322 @@ Definition with_context {a} (msg : string) (p : parser a) : parser a :=
     | inr y => inr y
     end.
 
-Definition parse {a} (parser : parser a) (input : string) : error_stack + a :=
-  fst <$> (parser input).
+#[program]
+Instance with_context_parser {a} (p : parser a) `{Parser a p} (msg : string)
+  : Parser (with_context msg p).
+
+Next Obligation.
+  unfold with_context.
+  destruct H as [is_parser].
+  specialize is_parser with input.
+  now destruct (p input).
+Qed.
+
+#[program]
+Instance with_context_strict {a} (p : parser a) `{StrictParser a p} (msg : string)
+  : StrictParser (with_context msg p).
+
+Next Obligation.
+  unfold with_context.
+  destruct H as [is_strict].
+  specialize is_strict with input.
+  now destruct (p input).
+Qed.
+
+Definition alt {a} (p q : parser a) : parser a :=
+  fun input =>
+    match p input with
+    | inr x => inr x
+    | inl _ => q input
+    end.
+
+Notation "p '<|>' q" := (alt p q) (at level 50, left associativity).
+
+#[program]
+Instance alt_strict {a} (p q : parser a) `{StrictParser a p} `{StrictParser a q}
+  : StrictParser (p <|> q).
+
+Next Obligation.
+  unfold alt.
+  destruct H as [is_strict_p].
+  destruct H0 as [is_strict_q].
+  specialize is_strict_p with input.
+  specialize is_strict_q with input.
+  now destruct (p input).
+Qed.
+
+#[program]
+Instance alt_parser {a} (p q : parser a) `{Parser a p} `{Parser a q}
+  : Parser (p <|> q).
+
+Next Obligation.
+  unfold alt.
+  destruct H as [is_parser_p].
+  destruct H0 as [is_parser_q].
+  specialize is_parser_p with input.
+  specialize is_parser_q with input.
+  now destruct (p input).
+Qed.
 
 Definition fail {a} (msg : string) : parser a :=
   fun s => inl (cons msg nil).
 
+#[program]
+Instance fail_strict {a} (msg : string) : StrictParser (@fail a msg).
+
 Definition read_char : parser ascii :=
   do var input <- get in
      match input with
-     | String a rst => do put rst;
-                          pure a
-                       end
+     | String a rst => put rst >> pure a
      | EmptyString => fail "expected character, found end of input"
      end
   end.
 
-Definition char (a : ascii) : parser unit :=
+#[program]
+Instance pure_Parser {a} (x : a) : Parser (pure x).
+
+#[program]
+Instance get_Parser : Parser get.
+
+#[program]
+Instance read_char_strict : StrictParser read_char.
+
+Next Obligation.
+  cbn.
+  destruct input.
+  + now cbn.
+  + cbn. lia.
+Qed.
+
+Definition char (a : ascii) : parser ascii :=
   do var c <- read_char in
      if eqb a c
-     then pure tt
+     then pure a
      else fail "expected a character, found another" (* todo: easy string interpolation *)
   end.
 
-Fixpoint str (a : string) : parser unit :=
-  let fix str_aux (a : string) :=
-      match a with
-      | String c rst => do char c;
-                           str_aux rst
-      end
-      | EmptyString => pure tt
-      end
-  in with_context "trying to consume a string" (str_aux a).
+#[program]
+Instance if_parser {a} (cond : bool) (p q : parser a)
+   `{Parser a p, Parser a q}
+  : Parser (if cond then p else q).
 
-Inductive iter_step (a b : Type) : Type :=
-| Continue (acc : a)
-| Return (res : b).
+Next Obligation.
+  destruct cond; apply (is_parser input).
+Qed.
 
-Arguments Continue [a b] (acc).
-Arguments Return [a b] (res).
+#[program]
+Remark char_strict (c : ascii) : StrictParser (char c).
+Proof.
+  typeclasses eauto.
+Qed.
 
-#[local]
-Fixpoint iter_aux {a b} (acc : a) (f : a -> ascii -> iter_step a b) (input : string)
-  : option (b * string) :=
-  match input with
-  | String c rst =>
-    match f acc c with
-    | Continue x => iter_aux x f rst
-    | Return b => Some (b, (String c rst))
-    end
-  | EmptyString => None
+Fixpoint str_aux (a : string) : parser unit :=
+  match a with
+  | String c rst => char c *> str_aux rst
+  | EmptyString => pure tt
   end.
 
-Definition iter {a b} (init : a) (f : a -> ascii -> iter_step a b) : parser b :=
-  do var input <- get in
-     match iter_aux init f input with
-     | Some (x, rst) =>
-       do put rst;
-          pure x
-        end
-     | None => fail "found end of input before satisfying a predicate"
-     end
+Instance str_aux_parser (s : string) : Parser (str_aux s).
+
+Proof.
+  induction s.
+  ++ apply pure_Parser.
+  ++ change (str_aux (String a s)) with (char a *> str_aux s).
+     apply bind_parser.
+     +++ typeclasses eauto.
+     +++ intros c.
+         apply IHs.
+Qed.
+
+Instance str_aux_strict (a : ascii) (s : string) : StrictParser (str_aux (String a s)).
+
+Proof.
+  change (str_aux (String a s)) with (char a *> str_aux s).
+  apply bind_strict_1; typeclasses eauto.
+Qed.
+
+Definition str (target : string) : parser string :=
+  with_context "trying to consume a string" (str_aux target) *> pure target.
+
+#[local, program]
+Fixpoint many_aux {a} (acc : list a) (p : parser a) `{StrictParser a p}
+    (input : string) {measure (length input)}
+  : list a * string :=
+  match p input with
+  | inl _ => (List.rev acc, input)
+  | inr (x, output) => many_aux (cons x acc) p output
   end.
 
-Definition until (continue : ascii -> bool) : parser string :=
-  do var cont <- iter id (fun (acc : string -> string) (c' : ascii) =>
-                            if continue c'
-                            then Return acc
-                            else Continue (fun (s : string) => acc (String c' s)))
-    in pure (cont EmptyString)
+Next Obligation.
+  destruct H as [is_strict].
+  specialize is_strict with input.
+  now rewrite <- Heq_anonymous in is_strict.
+Qed.
+
+Definition many {a} (p : parser a) `{StrictParser a p} : parser (list a) :=
+  fun (input : string) =>
+     match many_aux nil p input with
+     | (x, rst) => inr (x, rst)
+     end.
+
+#[program]
+Instance many_parser `{StrictParser a p} : Parser (many p).
+
+Next Obligation.
+  unfold many.
+  case_eq (many_aux nil p input); intros x rst equ.
+  (* TODO *)
+  admit.
+Admitted.
+
+Definition some {a} (p : parser a) `{StrictParser a p} : parser (list a) :=
+  do var x <- p in
+     var rst <- many p in
+     pure (cons x rst)
   end.
 
-Definition untilc (continue : ascii -> bool) : parser string :=
-  do var res <- until continue in
-     read_char;
-     pure res
+Remark some_parser `(StrictParser a p) : StrictParser p.
+typeclasses eauto.
+Qed.
+
+Definition whitespaces : parser (list ascii) :=
+  many (char " ").
+
+Remark whitespaces_parser : Parser whitespaces.
+typeclasses eauto.
+Qed.
+
+Definition ensure {a} (p : parser a) (cond : a -> bool) : parser a :=
+  do var res <- p in
+     if cond res
+     then pure res
+     else fail "ensure: result of p is not valid according to cond"
   end.
 
-Definition til_char (c : ascii) : parser string :=
-  until (eqb c).
+Remark ensure_parser `{Parser a p} (cond : a -> bool) : Parser (ensure p cond).
+typeclasses eauto.
+Qed.
 
-Definition til_charc (c : ascii) : parser string :=
-  untilc (eqb c).
+#[program]
+Fixpoint many_until_aux {a b} (acc : list a)
+    (p : parser a) `{StrictParser a p} (q : parser b)
+    (input : string) {measure (length input)}
+  : error_stack + (list a * string) :=
+    match q input with
+    | inl _ => match p input with
+               | inl _ => inl (cons "p failed before q could succeed"%string nil)
+               | inr (x, output) => many_until_aux (cons x acc) p q output
+               end
+    | inr (_, output) => inr (List.rev acc, output)
+    end.
 
-Definition whitespaces : parser unit :=
-  do until (fun c => negb (eqb c " "));
-     pure tt
-  end.
+Next Obligation.
+  admit.
+Admitted.
+
+Definition many_until {a b} (p : parser a) `{StrictParser a p} (q : parser b)
+  : parser (list a) :=
+  many_until_aux nil p q.
+
+#[program]
+Instance many_until_parser `(StrictParser a p, Parser b q) : Parser (many_until p q).
+
+Next Obligation.
+Admitted.
+
+#[program]
+Instance many_until_strict `(StrictParser a p, StrictParser b q) : StrictParser (many_until p q).
+
+Next Obligation.
+Admitted.
+
+Definition some_until {a b} (p : parser a) `{StrictParser a p} (q : parser b)
+  : parser (list a) :=
+  cons <$> p <*> many_until p q.
+
+#[program]
+Instance map_parser {a b} (f : a -> b) `(Parser a p) : Parser (f <$> p).
+
+Next Obligation.
+  unfold state_map.
+  case_eq (p input).
+  + now cbn.
+  + intros [x output] equ.
+    cbn.
+    destruct H as [is_parser].
+    specialize is_parser with input.
+    now rewrite equ in is_parser.
+Qed.
+
+#[program]
+Instance map_strict {a b} (f : a -> b) `(StrictParser a p) : StrictParser (f <$> p).
+
+Next Obligation.
+  unfold state_map.
+  case_eq (p input).
+  + now cbn.
+  + intros [x output] equ.
+    cbn.
+    destruct H as [is_strict].
+    specialize is_strict with input.
+    now rewrite equ in is_strict.
+Qed.
+
+#[program]
+Instance app_parser `(Parser (a -> b) f) `(Parser a p) : Parser (f <*> p).
+
+Next Obligation.
+  case_eq (f input).
+  + now cbn.
+  + intros [fp input'] equ.
+    assert (length input' <= length input). {
+      destruct H as [is_parser].
+      specialize is_parser with input.
+      now rewrite equ in is_parser.
+    }
+    cbn.
+    case_eq (p input').
+    ++ admit.
+    ++ admit.
+Admitted.
+
+#[program]
+Instance app_strict_1 `(StrictParser (a -> b) f, Parser a p) : StrictParser (f <*> p).
+
+Next Obligation.
+Admitted.
+
+#[program]
+Instance app_strict_2 `(Parser (a -> b) f, StrictParser a p) : StrictParser (f <*> p).
+
+Next Obligation.
+Admitted.
+
+Remark some_until_strict `(StrictParser a p, Parser b q) : StrictParser (some_until p q).
+typeclasses eauto.
+Qed.
+
+Definition eoi : parser unit :=
+  ensure (length <$> get) (Nat.eqb 0) >> pure tt.
+
+#[program]
+Instance eoi_parser : Parser eoi.
+
+Next Obligation.
+  induction input; now cbn.
+Qed.
+
+Definition peak {a} (p : parser a) : parser a :=
+  fun (input : string) =>
+    match p input with
+    | inl x => inl x
+    | inr (x, _) => inr (x, input)
+    end.
+
+#[program]
+Instance peak_parser {a} (p : parser a) : Parser (peak p).
+
+Next Obligation.
+  unfold peak.
+  destruct (p input) as [ _ | [x output] ]; auto.
+Qed.
