theories/HTTP.v
@@ -1,14 +1,52 @@
 From Praecia Require Import Parser.
 
-Definition http_request : parser (string * string) :=
-  do var method <- til_charc " " in
+Axiom of_ascii_list : list ascii -> string.
+
+Inductive directory_id : Type :=
+| Dirname (s : string)
+| Current
+| Parent.
+
+Inductive path := make_path { dirname : list directory_id
+                            ; filename : option string
+                            }.
+
+Definition dir_id_sep := peak (eoi <|> ((char " " <|> char "/") *> pure tt)).
+
+Definition dirid : parser directory_id :=
+  many (char "/") *>
+  (str ".." *> peak dir_id_sep *> pure Parent)
+  <|> (char "." *> peak dir_id_sep *> pure Current)
+  <|> (do var name <- some_until read_char (peak dir_id_sep) in
+          peak (char "/");
+          pure (Dirname (of_ascii_list name))
+       end).
+
+(* TODO: bad performance, can we provide some useful hints here? *)
+Definition path_dirname : parser (list directory_id) :=
+  many dirid.
+
+Eval vm_compute in (parse path_dirname "/../.salut////./tada").
+
+Definition read_path : parser path :=
+  do var dirname <- path_dirname in
+     many (char "/");
+     var maybe_filename <- many_until read_char (char " ") in
+     pure (make_path dirname (if Nat.eqb (List.length maybe_filename) 0
+                              then None
+                              else Some (of_ascii_list maybe_filename)))
+  end.
+
+Definition http_request : parser (string * path) :=
+  do var method <- str "GET" in
      whitespaces;
-     var path <- til_charc " " in
+     var path <- read_path in
      whitespaces;
-     str "HTTP/1.1"%string;
+     str "HTTP/1.1";
 
      pure (method, path)
   end.
 
 Eval vm_compute in (parse http_request "GET /etc/passwd HTTP/1.1"%string).
 Eval vm_compute in (parse http_request "GET /etc/passwd HTP/1.1"%string).
+Eval vm_compute in (parse http_request "PUT /etc/passwd HTTP/1.1"%string).
